

%%%
%%% CHAPTER
%%%
\section{Model Formulation}
 
%%% SUB-SECTION
\subsection{Mass Balance}
For a system with $n_{p}$ phases and $n_{c}$ components, the mass of each phase $j$ is,
\begin{equation}
m^{j} = \summation_{i=1}^{n_{c}}m_{i}^{j}\;\;\;\text{ for }j=1,2,\cdots,n_{p}
\label{Eqn_MassBalance_Phase}
\end{equation}

And the mass of each component $i\left(=1,2,\cdots,n_{c}\right)$,
\begin{equation}
m_{i} = m_{i}^{1} + m_{i}^{2} + \cdots + m_{i}^{n_{p}} = \summation_{j=1}^{n_{p}}m_{i}^{j}
\label{Eqn_MassBalance_Component}
\end{equation}

The total mass $m$ can be define as,
\begin{equation}
m - m^{1} + m^{2} + \cdots + m^{n_{p}} = \summation_{j=1}^{n_{p}}m^{j} = \summation_{i=1}^{n_{c}}m_{i}
\label{Eqn_MassBalance_Mass}
\end{equation}

Defining the intensive properties:
\begin{eqnarray}
w_{i}^{j} = \frc{m_{i}^{j}}{m^{j}} \label{Eqn_MassBalance_MassFraction} \\
z_{i} = \frc{m_{i}}{m} \label{Eqn_MassBalance_MassFractionFeeding} \\
\Pi^{j} = \frc{m^{j}}{m}\label{Eqn_MassBalance_PhaseMassFraction} 
\end{eqnarray}
where $w_{i}^{j}$ is the mass fraction of component $i$ in phase $j$, $\Pi^{j}$ is the mass fraction of phase $j$ and $z_{i}$ is the overall feed mass fraction of component $i$. From Eqns.~\ref{Eqn_MassBalance_Mass}-~\ref{Eqn_MassBalance_PhaseMassFraction}, we can define normalised quantities, i.e., fractions, and we can add the following constraints:
\begin{eqnarray}
&&w_{n_{c}}^{j} = 1 - \summation_{i=1}^{n_{c}-1}w_{i}^{j}  \hspace{3cm} j=1,2,\cdots,n_{p}  \label{Eqn_MassBalance_MassFraction2} \\
&&z_{n_{c}} = 1 - \summation_{i=1}^{n_{c}-1}z_{1}  \\
&&\Pi^{n_{p}} = 1 - \left(\Pi^{1} + \Pi^{2} + \cdots + \Pi^{n_{p}-1}\right) = 1 - \summation_{j=1}^{n_{p}-1} \Pi^{j}\label{Eqn_MassBalance_PhaseMassFraction2}
\end{eqnarray} 
with
\begin{displaymath}
  z_{i} = \frc{m_{i}}{m} = \frc{\summation_{j=1}^{n_{p}}m_{i}^{j}}{m} \frc{m^{j}}{m^{j}} = \underbrace{\frc{m^{j}}{m}}_{\red{\Pi^{j}}} \cdot \overbrace{\frc{\summation_{j=1}^{n_{p}}m_{i}^{j}}{m^{j}}}^{\red{\summation_{j=1}^{n_{p}}w_{i}^{j}}} 
\end{displaymath}
leading to
\begin{equation}
z_{i} = \Pi^{1}w_{i}^{1} + \Pi^{2}w_{i}^{2} + \cdots + \Pi^{n_{p}}w_{i}^{n_{p}}
\label{Eqn_MassBalance_FeedMassFractionConstraint}
\end{equation}
with
\begin{equation}
0\leq\Pi^{j}\leq 1 \hspace{3cm} 0\leq w_{i}^{j}\leq 1
\end{equation}

If the solution is contained within \red{$n_{p}$} phases, the inequality can be rewritten as,
\begin{equation}
0 < \Pi^{j} < 1
\end{equation}
Thus 
\begin{displaymath}
\Pi^{k} = 1 - \summation_{j=1,j\neq k}^{n_{p}} \Pi^{j} \neq 0
\end{displaymath}
Therefore from Eqn.~\ref{Eqn_MassBalance_FeedMassFractionConstraint},
\begin{equation}
w_{i}^{k} = \frc{z_{i}+\summation_{j=1,j\neq k}^{n_{p}}\Pi^{j}w_{i}^{j}}{\Pi^{k}} = \frc{z_{i} + \summation_{j=1,j\neq k}^{n_{p}}\Pi^{j}w_{i}^{j}}{1-\summation_{j=1,j\neq k}^{n_{p}}\Pi^{j}}
\label{Eqn_MassBalance_FeedMassFractionConstraint2}
\end{equation}


\begin{mdframed}[style=JFrame]
For 2 phases, $\Pi^{1}=L$ and $\Pi^{2}=V$, Eqn.~\ref{Eqn_MassBalance_FeedMassFractionConstraint} becomes:
\begin{displaymath}
w_{i}^{V} = \frc{z_{i}-Lw_{i}^{L}}{1-L}
\end{displaymath}
for $i=1,2,\cdots,n_{c}$, and for 3 phases,$\Pi^{1}=L$, $\Pi^{2}=V$ and $\Pi^{3}=H$:
\begin{displaymath}
w_{i}^{H} = \frc{z_{i}-\left(V w_{i}^{V} + L w_{i}^{L}\right)}{1 - \left(V w_{i}^{V} + L w_{i}^{L}\right)}
\end{displaymath}
\end{mdframed}

%% SUB-SECTION
\subsection{Free Gibbs Energy}
For equilibrium problems (e.g., vapour-liquid equilibrium, VLE), the total free Gibbs energy can be expressed as,
\begin{equation}
G = \summation_{j=1}^{n_{p}}\left(\summation_{i=1}^{n_{c}} m_{i}^{j}\mu_{i}^{j}\right)
\label{MassGibbs_Definition}
\end{equation} 
this represents
\begin{displaymath}
G = \summation_{i=1}^{n_{c}} m_{i}^{1}\mu_{i}^{1} + \summation_{i=1}^{n_{c}} m_{i}^{2}\mu_{i}^{2} + \cdots + \summation_{i=1}^{n_{c}} m_{i}^{n_{p}}\mu_{i}^{n_{p}}
\end{displaymath}
The chemical potential $\left(\mu\right)$ can be written as a function of the mass of each component at each phase,
\begin{eqnarray}
\mu_{i}^{j} &=& \mu_{i}^{j}\left(m_{1}^{j}, m_{2}^{j}, \cdots, m_{n_{c}}^{j}\right) = \mu_{i}^{j}\left(\frc{m_{1}^{j}}{m^{j}}, \frc{m_{2}^{j}}{m^{j}}, \cdots, \frc{m_{n_{c}}^{j}}{m^{j}}\right)\nonumber \\
 &=& \mu_{i}^{j}\left(w_{1}^{j}, w_{2}^{j}, \cdots, w_{n_{c}}^{j}\right)\label{chempotential_functional}
\end{eqnarray}
Dividing Eqn.~\ref{MassGibbs_Definition} by $m$,
\begin{equation}
g = \frc{G}{m} = \summation_{j=1}^{n_{p}}\left(\summation_{i=1}^{n_{c}}\frc{m_{i}^{j}}{m}\mu_{i}^{j}\right) = \summation_{i=1}^{n_{c}}\frc{m_{i}^{1}}{m^{1}} \cdot \frc{m^{1}}{m} \mu_{i}^{1} + \cdots + \summation_{i=1}^{n_{c}}\frc{m_{i}^{n_{p}}}{m^{n_{p}}} \cdot \frc{m^{n_{p}}}{m} \mu_{i}^{n_{p}}
\label{MassGibbs_Definition2}
\end{equation}
And we rewrite Eqn.~\ref{MassGibbs_Definition2} as,
\begin{equation}
g = \summation_{i=1}^{n_{c}}\Pi^{1}w_{i}^{1}\mu_{i}^{1} + \summation_{i=1}^{n_{c}}\Pi^{2}w_{i}^{2}\mu_{i}^{2} + \cdots + \summation_{i=1}^{n_{c}}\Pi^{n_{p}}w_{i}^{n_{p}}\mu_{i}^{n_{p}} = \summation_{j=1}^{n_{p}}\left[\summation_{i}^{n_{c}}\Pi^{j}w_{i}^{j}\mu_{i}^{j}\right] \label{MassGibbs_Definition3}
\end{equation}


\begin{mdframed}[style=JFrame]
For 2 ($L$ and $V$) phases,
\begin{displaymath}
g = \summation_{i=1}^{n_{c}}Lw_{i}^{L}\mu_{i}^{L} + \summation_{i=1}^{n_{c}}Vw_{i}^{V}\mu_{i}^{V}
\end{displaymath}
and 3 ($L$, $V$ and $H$) phases,
\begin{displaymath}
g = \summation_{i=1}^{n_{c}}Lw_{i}^{L}\mu_{i}^{L} + \summation_{i=1}^{n_{c}}Vw_{i}^{V}\mu_{i}^{V} + \summation_{i=1}^{n_{c}}Hw_{i}^{H}\mu_{i}^{H}
\end{displaymath}
\end{mdframed}


Now replacing Eqn.~\ref{Eqn_MassBalance_MassFraction2} in Eqn.~\ref{MassGibbs_Definition3},
\begin{equation}
g = \summation_{i=1}^{n_{c}-1}\Pi^{1}w_{i}^{1}\left(\mu_{i}^{1}-\mu_{n_{c}}^{1}\right) + \Pi^{1}\mu_{n_{c}}^{1} + \summation_{i=1}^{n_{c}-1}\Pi^{2}w_{i}^{2}\left(\mu_{i}^{2}-\mu_{n_{c}}^{2}\right) + \Pi^{2}\mu_{n_{c}}^{2} + \cdots + \summation_{i=1}^{n_{c}-1}\Pi^{n_{p}}w_{i}^{n_{p}}\left(\mu_{i}^{n_{p}}-\mu_{n_{c}}^{n_{p}}\right) + \Pi^{n_{p}}\mu_{n_{c}}^{n_{p}}
\label{MassGibbs_Definition4}
\end{equation}
Now replacing Eqns.~\ref{Eqn_MassBalance_PhaseMassFraction2} and~\ref{Eqn_MassBalance_FeedMassFractionConstraint2} in~\ref{MassGibbs_Definition4}:
\begin{eqnarray}
g &=& \summation_{i=1}^{n_{c}}\Pi^{1}w_{i}^{1}\left(\mu_{i}^{1}-\mu_{n_{c}}^{1}\right) + \Pi^{1}\mu_{n_{c}}^{1} + \cdots + \summation_{i=1}^{n_{c}}\Pi^{n_{p}-1}w_{i}^{n_{p}-1}\left(\mu_{i}^{n_{p}-1}-\mu_{n_{c}}^{n_{p}-1}\right) + \Pi^{n_{p}-1}\mu_{n_{c}}^{n_{p}-1} + \nonumber \\
   && \summation_{i=1}^{n_{c}-1}\left[z_{i} - \summation_{j=1}^{n_{p}-1}\Pi^{j}w_{i}^{j}\right]\left(\mu_{i}^{n_{p}}-\mu_{n_{c}}^{n_{p}}\right) + \Pi^{n_{p}}\mu_{n_{c}}^{n_{p}}\nonumber
\end{eqnarray}

Rearranging
\begin{eqnarray}
g &=& \summation_{i=1}^{n_{c}}\Pi^{1}w_{i}^{1}\left[\left(\mu_{i}^{1}-\mu_{i}^{n_{p}}\right) - \left(\mu_{n_{c}}^{1}-\mu_{n_{c}}^{n_{p}}\right)\right] + \cdots + \summation_{i=1}^{n_{c}}\Pi^{n_{p}-1}w_{i}^{n_{p}-1}\left[\left(\mu_{i}^{n_{p}-1}-\mu_{i}^{n_{p}}\right) - \left(\mu_{n_{c}}^{n_{p}-1}-\mu_{n_{c}}^{n_{p}}\right)\right] + \nonumber \\
&& \summation_{j=1}^{n_{p}-1}\Pi^{j}\mu_{n_{c}}^{j} + \summation_{i=1}^{n_{c}-1}z_{i}\left(\mu_{i}^{n_{p}}-\mu_{n_{c}}^{n_{p}}\right) +\left(1-\summation_{j=1}^{n_{p}-1}\Pi^{j}\right)\mu_{n_{c}}^{n_{p}} \nonumber
\end{eqnarray}

With a compressed notation:

\begin{eqnarray}
g &=& \summation_{i=1}^{n_{c}-1}\left\{\summation_{j=1}^{n_{p}-1}\Pi^{j}w_{i}^{j}\left[\left(\mu_{i}^{j}-\mu_{i}^{n_{p}}\right) - \left(\mu_{n_{c}}^{j}-\mu_{n_{c}}^{n_{p}}\right)\right]\right\} + \summation_{j=1}^{n_{p}-1}\Pi^{j}\left(\mu_{n_{c}}^{j}-\mu_{n_{c}}^{n_{p}}\right) +  \nonumber \\
&& \hspace{3cm} \summation_{i=1}^{n_{c}-1} z_{i}\mu_{i}^{n_{p}} + \underbrace{\left(1-\summation_{i=1}^{n_{c}-1}z_{i}\right)}_{\red{z_{n_{c}}}}\mu_{n_{c}}^{n_{p}} \nonumber 
\end{eqnarray}
Thus
\red{\begin{equation}
g = \summation_{i=1}^{n_{c}-1}\left\{\summation_{j=1}^{n_{p}-1}\Pi^{j}w_{i}^{j}\left[\left(\mu_{i}^{j}-\mu_{i}^{n_{p}}\right) - \left(\mu_{n_{c}}^{j}-\mu_{n_{c}}^{n_{p}}\right)\right]\right\} + \summation_{j=1}^{n_{p}-1}\Pi^{j}\left(\mu_{n_{c}}^{j}-\mu_{n_{c}}^{n_{p}}\right) + \summation_{i=1}^{n_{c}}z_{i}\mu_{i}^{n_{p}}
\end{equation}}

The chemical potential was defined as a functional (Eqn.~\ref{chempotential_functional}):
\begin{eqnarray}
&& \mu_{i}^{1} = \mu_{i}^{1}\left(w_{1}^{1},w_{2}^{1},\cdots,w_{n_{c}}^{1}\right) \nonumber \\
&& \mu_{i}^{2} = \mu_{i}^{2}\left(w_{1}^{2},w_{2}^{2},\cdots,w_{n_{c}}^{2}\right) \nonumber \\
&& \hspace{2cm}\vdots \nonumber \\
&& \mu_{i}^{n_{p}} = \mu_{i}^{n_{p}}\left(w_{1}^{n_{p}},w_{2}^{n_{p}},\cdots,w_{n_{c}}^{n_{p}}\right) \label{ChemPotDef2}
\end{eqnarray}
with constraint Eqn.~\ref{Eqn_MassBalance_FeedMassFractionConstraint2} in Eqn.~\ref{ChemPotDef2},
\begin{eqnarray}
\mu_{l}^{k} &=& \mu_{l}^{k}\left(w_{i}^{j},\Pi^{j}\right) \nonumber \\
           &=& \mu_{l}^{k}\left(w_{1}^{1},\cdots,w_{n_{c}-1}^{1},w_{1}^{2},\cdots,w_{n_{c}-1}^{2},\cdots,w_{1}^{n_{p}},w_{2}^{n_{p}},\cdots,w_{n_{c}-1}^{n_{p}},\Pi^{1},\cdots,\Pi^{n_{p}}\right)\nonumber
\end{eqnarray}
with $i = 1, 2, \cdots, l, \cdots, n_{c} - 1$, $j = 1, 2, \cdots, n_{p}$ and $j\neq k$

And the mass-based free Gibbs energy should take the following format
\begin{displaymath}
g = g\left(w_{i}^{j},\Pi^{j}\right).
\end{displaymath}
From classical thermodynamic, $\mu_{i}^{j}$ can be defined as a function of the fugacity coefficient, $\varphi_{i}^{j}$,
\begin{equation}
\mu_{i}^{j}= R T\left[\ln\varphi_{i}^{j} + \ln\left(P x_{i}^{j}\right)\right] + \theta_{i}\left(T\right),
\end{equation}
where $\theta_{i}$ is an integration constant. The fugacity coefficient is defined as,
\begin{equation}
\varphi_{i}^{j} = \frc{f_{i}^{j}}{P x_{i}^{j}},
\end{equation}
where $f$ and $x$ are the fugacity and molar fraction respectively.


